Simplify first online model (#13)
* simplified first model of the online? protocol

* small adaptions to better match two-message and online model

* twomessage: changed state tag

* online protocol: simplified key setup (hiding LongTermPkeKey constructor)

* simplified printing of PKE keys (overwriting default_trace_to_string_printers in DY.Simplified)

* minor cleanup to match tutorial text

* unifying 'Two-Message protocol'

* minor cleanup

* use tutorial makefile for DY* extensions

* Revert "minor cleanup"

This reverts commit be1e17311f447ef5e1e6586c540f5a5c306c8ba6.

* remove global key session IDs (as they are no longer used)

dy-extensions/DY.Simplified.fst
@@ -147,3 +147,89 @@ let bytes_invariant_pke_dec_with_key_lookup tr #a alice keys_sid key_tag cipher 
       bytes_invariant_pke_dec tr sk_alice sk_usg cipher;
       serialize_parse_inv_lemma a cipher_dec
   )
+
+
+
+// generate a private LongTermPkeKey with a given tag
+// (this hides the LongTermPkeKey constructor from the user)
+val generate_private_pke_key: principal -> state_id -> string -> traceful (option unit)
+let generate_private_pke_key prin private_keys_sid key_tag =
+  generate_private_key prin private_keys_sid (LongTermPkeKey key_tag)
+
+
+// Store Bob's public Pke key in Alice's state
+// Bob's public key is computed from his private key
+// 1. Retrieve Bob's private key from his private key session (using the tag)
+// 2. Compute the public key from the private key
+// 3. Install Bob's public key in Alice's public key store (under the same tag)
+val install_public_pke_key:
+  (alice:principal) -> (alice_public_keys_sid:state_id) ->
+  (key_tag:string) ->
+  (bob:principal) -> (bob_private_keys_sid:state_id) ->
+  traceful (option unit)
+let install_public_pke_key alice alice_public_keys_sid key_tag bob bob_private_keys_sid =
+  let*? priv_key_bob = get_private_key bob bob_private_keys_sid (LongTermPkeKey key_tag) in
+  let pub_key_bob = pk priv_key_bob in
+  install_public_key alice alice_public_keys_sid (LongTermPkeKey key_tag) bob pub_key_bob
+
+
+
+(*** Printing PkeKeys ***)
+
+(* For the first example protocol using public key encryption (the Online? protocol),
+   I want a simple to understand printing of the trace.
+
+   The following functions simplify printing of Pke Keys:
+   * The LongTermPkeKey constructor is hidden
+   * For public keys, the lookup key for the dictionary is written as pair 
+     (of key tag and principal)
+*)
+
+val long_term_key_type_to_string_: DY.Lib.State.PrivateKeys.long_term_key_type -> string
+let long_term_key_type_to_string_ t =
+  match t with
+  | DY.Lib.State.PrivateKeys.LongTermPkeKey u -> u
+  | DY.Lib.State.PrivateKeys.LongTermSigKey u -> "LongTermSigKey " ^ u
+
+val private_keys_types_to_string_: (list (map_elem DY.Lib.State.PrivateKeys.private_key_key DY.Lib.State.PrivateKeys.private_key_value)) -> string
+let rec private_keys_types_to_string_ m =
+  match m with
+  | [] -> ""
+  | hd :: tl -> (
+    (private_keys_types_to_string_ tl) ^ 
+    Printf.sprintf "%s = (%s)," (long_term_key_type_to_string_ hd.key.ty) (bytes_to_string hd.value.private_key)
+  )
+
+val private_keys_state_to_string: bytes -> option string
+let private_keys_state_to_string content_bytes =
+  let? state = parse (map DY.Lib.State.PrivateKeys.private_key_key DY.Lib.State.PrivateKeys.private_key_value) content_bytes in
+  Some (Printf.sprintf "[%s]" (private_keys_types_to_string_ state.key_values))
+
+
+
+val pki_types_to_string: (list (map_elem DY.Lib.State.PKI.pki_key DY.Lib.State.PKI.pki_value)) -> string
+let rec pki_types_to_string m =
+  match m with
+  | [] -> ""
+  | hd :: tl -> (
+    (pki_types_to_string tl) ^ 
+    Printf.sprintf "(%s, %s) = (%s)," (long_term_key_type_to_string_ hd.key.ty) hd.key.who (bytes_to_string hd.value.public_key)
+  )
+  
+val pki_state_to_string: bytes -> option string
+let pki_state_to_string content_bytes =
+  let? state = parse (map DY.Lib.State.PKI.pki_key DY.Lib.State.PKI.pki_value) content_bytes in
+  Some (Printf.sprintf "[%s]" (pki_types_to_string state.key_values))
+
+let default_pke_keys_printer =
+ [ (DY.Lib.State.PrivateKeys.map_types_private_keys.tag, private_keys_state_to_string)
+ ; (DY.Lib.State.PKI.map_types_pki.tag, pki_state_to_string)
+ ]
+
+let default_state_to_string = default_pke_keys_printer
+
+let default_trace_to_string_printers =
+  trace_to_string_printers_builder 
+    default_message_to_string
+    default_state_to_string
+    default_event_to_string
