examples/Online/DY.Online.Protocol.fst
@@ -10,7 +10,7 @@ open DY.Extend
 open DY.Online.Data
 
 /// Here we define the DY* mode of the "Online?" protocol,
-/// an extension of the simple Two Message protocol:
+/// an extension of the simple Two-Message protocol:
 /// the two messages are now (asymmetrically) encrypted
 ///
 /// A -> B: enc{Ping (A, n_A)}_B
@@ -18,13 +18,12 @@ open DY.Online.Data
 ///
 /// The model consists of 3 functions,
 /// one for each protocol step
-/// (just as for the simple two message protocol):
+/// (just as for the simple Two-Message protocol):
 /// 1. Alice sends the Ping to Bob (`send_ping`)
 /// 2. Bob receives the Ping and replies with the Ack (`receive_ping_and_send_ack`)
 /// 3. Alice receives the Ack (`receive_ack`)
 ///
-/// Additionally, there are two helper functions
-/// for steps 2 and 3 (`decode_ping` and `decode_ack`).
+/// We highlight the differences to the model of the Two-Message protocol.
 
 (*** Sending the Ping ***)
 
@@ -39,17 +38,23 @@ open DY.Online.Data
 /// encryption was not successful, i.e.,
 /// Alice does not have a public key of Bob.
 
-let nonce_label alice bob = join (principal_label alice) (principal_label bob)
-
 val send_ping: principal -> principal -> state_id -> traceful (option (state_id & timestamp))
-let send_ping alice bob keys_sid =
-  // TODO: explain high-level idea of "intended readers"
-  let* n_a = gen_rand_labeled (nonce_label alice bob) in
+let send_ping alice bob alice_public_keys_sid =
+  let* n_a = gen_rand in
   
   let ping = Ping {alice; n_a} in 
 
-  // encrypt the message for bob
-  let*? ping_encrypted = pke_enc_for alice bob keys_sid key_tag ping in
+  (* Instead of just serializing the message,
+     (as in the Two-Message Protocol model),
+     we need to encrypt the Ping for Bob,
+     using a public key of Bob with the protocol tag
+     stored in Alice's public key storage.
+
+     (may fail, Alice doesn't have a public key
+     for Bob with the right tag stored in her key session)
+    *)
+  // returns the cipher text in wire format (i.e., includes serializing)
+  let*? ping_encrypted = pke_enc_for alice bob alice_public_keys_sid key_tag ping in
   let* msg_ts = send_msg ping_encrypted in
 
   let ping_state = SentPing {bob; n_a} in
@@ -72,47 +77,41 @@ let send_ping alice bob keys_sid =
 /// The step fails, if one of
 /// * decryption fails
 /// * the message is not of the right type, i.e., not a first message
-/// * encryption fails
+/// * encryption fails (for example, if Bob doesn't have a public key for Alice)
 
-/// Decrypting the message (Step 2 from above) is pulled out to a separate function
-/// The function
-/// * decrypts the message
-/// * checks that the message is of the right type (a Ping)
-/// * returns the content of the message
-/// The function fails if decryption fails.
-
-val decode_ping : principal -> state_id -> bytes -> traceful (option ping_t)
-let decode_ping bob keys_sid msg =
-  // try to decrypt the message with
-  // a private key of bob with the protocol tag
-  // (fails, if no such key exists)
-  let*? png = pke_dec_with_key_lookup #message_t bob keys_sid key_tag msg in
-  
-  // check that the decrypted message is of the right type
-  // (otherwise fail)
-  guard_tr (Ping? png);*?
-
-  // return the content of the message 
-  // (i.e., strip the Ping constructor)
-  return (Some (Ping?.ping png))
-
-/// Now the actual receive and reply step
-/// using the decode function
-val receive_ping_and_send_ack: principal -> global_sess_ids -> timestamp -> traceful (option (state_id & timestamp))
-let receive_ping_and_send_ack bob global_sids msg_ts =
+val receive_ping_and_send_ack: principal -> state_id -> state_id -> timestamp -> traceful (option (state_id & timestamp))
+let receive_ping_and_send_ack bob bob_private_keys_sid bob_public_keys_sid msg_ts =
   let*? msg = recv_msg msg_ts in
-  // decode the received expected ping
-  let*? png = decode_ping bob global_sids.private_keys msg in
 
-  let n_a = png.n_a in
+  (* Instead of just parsing the message msg
+     (as in the Two-Message Protocol model),
+     we now have to decrypt the received message
+     with a private key of Bob having the protocol tag.
+     (fails, if no such key exists)
+  *)
+  // returns the abstract message (i.e., includes parsing)
+  let*? png_ = pke_dec_with_key_lookup #message_t bob bob_private_keys_sid key_tag msg in
+
+  guard_tr (Ping? png_);*?
+
+  let Ping png = png_ in
   let alice = png.alice in
+  let n_a = png.n_a in
 
   let ack = Ack {n_a} in
-  // encrypt the reply for alice
-  let*? ack_encrypted = pke_enc_for bob alice global_sids.pki key_tag ack in
+
+  (* Instead of just serializing the message,
+     (as in the Two-Message Protocol model),
+     we need to encrypt it for Alice,
+     using a public key of Alice with the protocol tag
+     stored in Bob's public key storage.
+  *)
+  let*? ack_encrypted = pke_enc_for bob alice bob_public_keys_sid key_tag ack in
+
   let* ack_ts = send_msg ack_encrypted in
-  
-  let* sess_id = start_new_session bob (SentAck {alice; n_a}) in
+
+  let ack_state = SentAck {alice; n_a} in
+  let* sess_id = start_new_session bob ack_state in
   
   return (Some (sess_id, ack_ts))
 
@@ -131,37 +130,29 @@ let receive_ping_and_send_ack bob global_sids msg_ts =
 /// * the message is not of the right type, i.e., not a reply
 /// * there is no prior session related to n_a
 
+val receive_ack: principal -> state_id -> timestamp -> traceful (option state_id)
+let receive_ack alice alice_private_keys_sid ack_ts =
+  let*? msg = recv_msg ack_ts in
 
-/// Again, we pull out decryption of the message (Step 2):
-/// * decrypt the message
-/// * check that the message is of the Ack type
-/// Returns the content of the reply.
-/// Fails if decryption fails.
+  (* Instead of just parsing the message msg
+     (as in the Two-Message Protocol model),
+     we now have to decrypt the received message
+     with a private key of Alice having the protocol tag.
+     (fails, if no such key exists)
+  *)
+  // returns the abstract message (i.e., includes parsing)
+  let*? ack = pke_dec_with_key_lookup #message_t alice alice_private_keys_sid key_tag msg in
 
-val decode_ack : principal -> state_id -> bytes -> traceful (option ack_t)
-let decode_ack alice keys_sid cipher =
-  // try to decrypt the message with
-  // a private key of alice with the protocol tag
-  let*? ack = pke_dec_with_key_lookup #message_t alice keys_sid key_tag cipher in
-
-  // check that the decrypted message is of the Ack type
   guard_tr (Ack? ack);*?
 
-  // return the content of the message
-  return (Some (Ack?.ack ack))
-
-/// The actual protocol step using the decode function
-val receive_ack: principal -> state_id -> timestamp -> traceful (option state_id)
-let receive_ack alice keys_sid ack_ts =
-  let*? msg = recv_msg ack_ts in
-  // decode the received expected ack
-  let*? ack = decode_ack alice keys_sid msg in
-
+  let Ack ack = ack in
   let n_a = ack.n_a in
 
   let*? (st, sid) = lookup_state #state_t alice
-    (fun st -> SentPing? st && (SentPing?.ping st).n_a = n_a)
-    in
+    (fun st -> 
+          SentPing? st
+      && (SentPing?.ping st).n_a = n_a
+    ) in
   guard_tr(SentPing? st);*?
   let bob = (SentPing?.ping st).bob in
 
