examples/Online/DY.Online.Run.fst
@@ -3,6 +3,8 @@ module DY.Online.Run
 open DY.Core
 open DY.Lib
 
+open DY.Simplified
+
 open DY.Online.Run.Printing
 open DY.Online.Data
 open DY.Online.Protocol
@@ -23,52 +25,33 @@ let run () : traceful (option unit ) =
 
   // Initialize key storage for Alice
   // private and public keys are stored in separate sessions
-  let* alice_priv_keys_sid = initialize_private_keys alice in
-  let* alice_pub_keys_sid = initialize_pki alice in
-  // we collect both session ids in a global record
-  let alice_global_session_ids : global_sess_ids = 
-    { pki = alice_pub_keys_sid; 
-      private_keys = alice_priv_keys_sid
-    } in
+  let* alice_private_keys_sid = initialize_private_keys alice in
+  let* alice_public_keys_sid = initialize_pki alice in
 
   // Initialize key storage for Bob
-  let* bob_priv_keys_sid = initialize_private_keys bob in
-  let* bob_pub_keys_sid = initialize_pki bob in  
-  let bob_global_session_ids: global_sess_ids = 
-    { pki = bob_pub_keys_sid; 
-      private_keys = bob_priv_keys_sid
-    } in
+  let* bob_private_keys_sid = initialize_private_keys bob in
+  let* bob_public_keys_sid = initialize_pki bob in  
 
   // Generate private key for Alice and store it in her private keys session
-  generate_private_key alice alice_global_session_ids.private_keys (LongTermPkeKey key_tag);*
+  generate_private_pke_key alice alice_private_keys_sid key_tag;*
   
   // Generate private key for Bob and store it in his private keys session
-  generate_private_key bob bob_global_session_ids.private_keys (LongTermPkeKey key_tag);*
+  generate_private_pke_key bob bob_private_keys_sid key_tag;*
 
   // Store Bob's public key in Alice's state
-  // Bob's public key is computed from his private key
-  // 1. Retrieve Bob's private key from his private key session
-  // 2. Compute the public key from the private key
-  // 3. Install Bob's public key in Alice's public key store
-  let*? priv_key_bob = get_private_key bob bob_global_session_ids.private_keys (LongTermPkeKey key_tag) in
-  let pub_key_bob = pk priv_key_bob in
-  install_public_key alice alice_global_session_ids.pki (LongTermPkeKey key_tag) bob pub_key_bob;*
+  install_public_pke_key alice alice_public_keys_sid key_tag bob bob_private_keys_sid;*
 
-  // Store Alice's public key in Bob's state in the same way
-  let*? priv_key_alice = get_private_key alice alice_global_session_ids.private_keys (LongTermPkeKey key_tag) in
-  let pub_key_alice = pk priv_key_alice in
-  install_public_key bob bob_global_session_ids.pki (LongTermPkeKey key_tag) alice pub_key_alice;*
-
-
+  // Store Alice's public key in Bob's state
+  install_public_pke_key bob bob_public_keys_sid key_tag alice alice_private_keys_sid;*
 
   (*** The actual protocol run ***)
 
   // Alice sends a Ping to Bob
-  let*? (alice_sid, ping_ts) = send_ping alice bob alice_global_session_ids.pki in
+  let*? (alice_sid, ping_ts) = send_ping alice bob alice_public_keys_sid in
   // Bob replies with an Ack (reading the ping at the given timestamp)
-  let*? (bob_sid, ack_ts) = receive_ping_and_send_ack bob bob_global_session_ids ping_ts in
+  let*? (bob_sid, ack_ts) = receive_ping_and_send_ack bob bob_private_keys_sid bob_public_keys_sid ping_ts in
   // Alice receives the Ack (at the given ack timestamp)
-  let*? _ = receive_ack alice alice_global_session_ids.private_keys ack_ts in
+  receive_ack alice alice_private_keys_sid ack_ts;*?
 
 
  (*** Printing the Trace ***)
