examples/TwoMessageP/DY.TwoMessage.Run.fst
@@ -2,11 +2,12 @@ module DY.TwoMessage.Run
 
 open DY.Core
 open DY.Lib
+open DY.Simplified
 
 open DY.TwoMessage.Run.Printing
 open DY.TwoMessage.Protocol
 
-/// Here, we print the trace after a successful run of the Two Message protocol.
+/// Here, we print the trace after a successful run of the Two-Message protocol.
 
 let run () : traceful (option unit ) =
   let _ = IO.debug_print_string "************* Trace *************\n" in
@@ -29,7 +30,7 @@ let run () : traceful (option unit ) =
 
   // Alice receives the Ack
   // (we pass the timestamp of Bob's response to the receive function of Alice)
-  let*? _ = receive_ack alice ack_ts in
+  receive_ack alice ack_ts;*?
 
 
   (*** Printing the Trace ***)
